logrel_unary.v
@@ -7,73 +7,325 @@ Import uPred.
 
 Definition logN : namespace := nroot .@ "logN".
 
+Record domain_func (A B : ofeT) : Type := DomainFunc {
+  domain_func_car :> A → B;
+  domain_func_is_strongly_contractive : bool;
+  domain_func_maybe_contractive :
+    if domain_func_is_strongly_contractive then
+      Contractive domain_func_car
+    else
+      NonExpansive domain_func_car
+}.
+Arguments DomainFunc {_ _} _ {_}.
+Arguments domain_func_is_contractive {_ _} _.
+Arguments domain_func_maybe_contractive {_ _} _.
+Add Printing Constructor domain_func.
+Global Instance domain_func_ne {A B} (f : domain_func A B) : NonExpansive f.
+Proof.
+  destruct f as [f [] Hf]; last done.
+  by apply contractive_ne.
+Qed.
+
+Notation "'λdfne' x .. y , t" :=
+  (@DomainFunc _ _ (λ x, .. (@DomainFunc _ _ (λ y, t) false _) ..) false _)
+  (at level 200, x binder, y binder, right associativity).
+
+Notation "'λdfco' x .. y , t" :=
+  (@DomainFunc _ _ (λ x, .. (@DomainFunc _ _ (λ y, t) true _) ..) true _)
+  (at level 200, x binder, y binder, right associativity).
+
+Section domain_func.
+  Context {A B : ofeT}.
+  Global Instance ofe_contr_mor_proper
+         (f : domain_func A B) : Proper ((≡) ==> (≡)) f.
+  Proof. apply ne_proper; apply _. Qed.
+  Instance domain_func_equiv : Equiv (domain_func A B) := λ f g, ∀ x, f x ≡ g x.
+  Instance domain_func_dist : Dist (domain_func A B) := λ n f g, ∀ x, f x ≡{n}≡ g x.
+  Definition domain_func_ofe_mixin : OfeMixin (domain_func A B).
+  Proof.
+    split.
+    - intros f g; split; [intros Hfg n k; apply equiv_dist, Hfg|].
+      intros Hfg k; apply equiv_dist=> n; apply Hfg.
+    - intros n; split.
+      + by intros f x.
+      + by intros f g ? x.
+      + by intros f g h ?? x; trans (g x).
+    - by intros n f g ? x; apply dist_S.
+  Qed.
+  Canonical Structure domain_funcO :=
+    OfeT (domain_func A B) domain_func_ofe_mixin.
+
+  Program Definition domain_func_chain (c : chain domain_funcO)
+    (x : A) : chain B := {| chain_car n := c n x |}.
+  Next Obligation. intros c x n i ?. by apply (chain_cauchy c). Qed.
+  Program Definition domain_func_compl `{Cofe B} : Compl domain_funcO := λ c,
+    λdfne x, compl (domain_func_chain c x).
+  Next Obligation.
+    intros ? c n x y Hx.
+      by rewrite (conv_compl n (domain_func_chain c x))
+                 (conv_compl n (domain_func_chain c y)) /= Hx.
+  Qed.
+  Global Program Instance domain_func_cofe `{Cofe B} : Cofe domain_funcO :=
+    {| compl := domain_func_compl |}.
+  Next Obligation.
+    intros ? n c x; simpl.
+    by rewrite (conv_compl n (domain_func_chain c x)) /=.
+  Qed.
+
+  Global Instance domain_func_mor_car_ne :
+    NonExpansive2 (@domain_func_car A B).
+  Proof. intros n f g Hfg x y Hx. rewrite Hx; apply Hfg. Qed.
+  Global Program Instance domain_func_car_proper :
+    Proper ((≡) ==> (≡) ==> (≡)) (@domain_func_car A B) := ne_proper_2 _.
+  Lemma domain_func_ext (f g : domain_func A B) : f ≡ g ↔ ∀ x, f x ≡ g x.
+  Proof. done. Qed.
+End domain_func.
+
+Arguments domain_funcO : clear implicits.
+
+Notation "A -df> B" :=
+  (domain_funcO A B) (at level 99, B at level 200, right associativity).
+
+Instance ofe_contr_mor_inhabited {A B : ofeT} `{Inhabited B} :
+  Inhabited (A -df> B) := populate (λdfne _, inhabitant).
+Proof. solve_proper. Defined.
+
+Program Definition cconst_contr {A B : ofeT} : B → A -df> B := λ x, λdfne _, x.
+Next Obligation.
+Proof. by intros ???????. Qed.
+
+Record domain_mor (A : ofeT) Σ : Type := DomainMor {
+  domain_mor_car :> A → iProp Σ;
+  domain_mor_ne : NonExpansive domain_mor_car;
+  domain_mor_persistent : ∀ x, Persistent (domain_mor_car x)
+}.
+Arguments DomainMor {_ _} _ {_}.
+Arguments domain_mor_car {_ _} _.
+Add Printing Constructor domain_mor.
+Existing Instance domain_mor_ne.
+Existing Instance domain_mor_persistent.
+
+Notation "'λdo' x .. y , t" :=
+  (@DomainMor _ _ (λ x, .. (@DomainMor _ _ (λ y, t) _ _) ..) _ _)
+  (at level 200, x binder, y binder, right associativity).
+
+Section domain_mor.
+  Context {A : ofeT} {Σ : gFunctors}.
+  Global Instance domain_mor_proper
+         (f : domain_mor A Σ) : Proper ((≡) ==> (≡)) f.
+  Proof. apply ne_proper; apply _. Qed.
+  Instance domain_mor_equiv : Equiv (domain_mor A Σ) := λ f g, ∀ x, f x ≡ g x.
+  Instance domain_mor_dist : Dist (domain_mor A Σ) := λ n f g, ∀ x, f x ≡{n}≡ g x.
+  Definition domain_mor_ofe_mixin : OfeMixin (domain_mor A Σ).
+  Proof.
+    split.
+    - intros f g; split; [intros Hfg n k; apply equiv_dist, Hfg|].
+      intros Hfg k; apply equiv_dist=> n; apply Hfg.
+    - intros n; split.
+      + by intros f x.
+      + by intros f g ? x.
+      + by intros f g h ?? x; trans (g x).
+    - by intros n f g ? x; apply dist_S.
+  Qed.
+  Canonical Structure domain_morO :=
+    OfeT (domain_mor A Σ) domain_mor_ofe_mixin.
+
+  Local Arguments uPred_holds _ !_ _ _.
+
+  Program Definition domain_mor_chain (c : chain domain_morO)
+    (x : A) : chain (iProp Σ) := {| chain_car n := c n x |}.
+  Next Obligation. intros c x n i ?. by apply (chain_cauchy c). Qed.
+  Program Definition domain_mor_compl : Compl domain_morO := λ c,
+    λdo x, compl (domain_mor_chain c x).
+  Next Obligation.
+    intros c n x y Hx.
+      by rewrite (conv_compl n (domain_mor_chain c x))
+                 (conv_compl n (domain_mor_chain c y)) /= Hx.
+  Qed.
+  Next Obligation. (* How can we prove this in the logic!? *)
+  Proof.
+    intros ??.
+    constructor => n z Hz.
+    unseal; rewrite /uPred_persistently_def /=.
+    intros Hx.
+    apply (conv_compl n (domain_mor_chain c x)); auto using cmra_core_validN.
+    apply (symmetry (conv_compl n (domain_mor_chain c x))) in Hx;
+      auto using cmra_core_validN.
+    simpl in *.
+    destruct (domain_mor_persistent _ _ (c n) x) as [Hpr].
+    revert Hpr; unseal; intros Hpr.
+    by apply Hpr.
+  Qed.
+
+  Global Program Instance domain_mor_cofe : Cofe domain_morO :=
+    {| compl := domain_mor_compl |}.
+  Next Obligation.
+    intros n c x; simpl.
+    by rewrite (conv_compl n (domain_mor_chain c x)) /=.
+  Qed.
+
+
+  Global Instance domain_mor_car_ne :
+    NonExpansive2 (@domain_mor_car A Σ).
+  Proof. intros n f g Hfg x y Hx; rewrite Hx; apply Hfg. Qed.
+  Global Instance domain_mor_car_proper :
+    Proper ((≡) ==> (≡) ==> (≡)) (@domain_mor_car A Σ) := ne_proper_2 _.
+  Lemma dmain_mor_ext (f g : domain_mor A Σ) : f ≡ g ↔ ∀ x, f x ≡ g x.
+  Proof. done. Qed.
+End domain_mor.
+
+Arguments domain_morO : clear implicits.
+
+Notation "A -d> B" :=
+  (domain_morO A B) (at level 99, B at level 200, right associativity).
+
+Instance domain_mor_inhabited {A : ofeT} {Σ : gFunctors} :
+  Inhabited (A -d> Σ) := populate (λdo _, inhabitant)%I.
+
+Program Definition true_domain {A : ofeT} {Σ : gFunctors} : A -d> Σ := λdo _, True%I.
+
 (** interp : is a unary logical relation. *)
 Section logrel.
   Context `{heapIG Σ}.
-  Notation D := (valO F_mu_ref_conc_lang -n> iProp Σ).
+  Notation D := (valO F_mu_ref_conc_lang -d> Σ).
   Implicit Types τi : D.
   Implicit Types Δ : listO D.
-  Implicit Types interp : listO D → D.
+  Implicit Types interp : listO D -df> D.
 
-  Program Definition env_lookup (x : var) : listO D -n> D := λne Δ,
-    from_option id (cconst False)%I (Δ !! x).
-  Solve Obligations with solve_proper.
-
-  Definition interp_top : listO D -n> D := λne Δ w, True%I.
-
-  Program Definition interp_unit : listO D -n> D := λne Δ w, ⌜w = UnitV⌝%I.
-  Program Definition interp_nat : listO D -n> D := λne Δ w, ⌜∃ n, w = #nv n⌝%I.
-  Program Definition interp_bool : listO D -n> D := λne Δ w, ⌜∃ n, w = #♭v n⌝%I.
-
-  Program Definition interp_prod
-      (interp1 interp2 : listO D -n> D) : listO D -n> D := λne Δ w,
-    (∃ w1 w2, ⌜w = PairV w1 w2⌝ ∧ interp1 Δ w1 ∧ interp2 Δ w2)%I.
-  Solve Obligations with repeat intros ?; simpl; solve_proper.
-
-  Program Definition interp_sum
-      (interp1 interp2 : listO D -n> D) : listO D -n> D := λne Δ w,
-    ((∃ w1, ⌜w = InjLV w1⌝ ∧ interp1 Δ w1) ∨ (∃ w2, ⌜w = InjRV w2⌝ ∧ interp2 Δ w2))%I.
-  Solve Obligations with repeat intros ?; simpl; solve_proper.
-
-  Program Definition interp_arrow
-      (interp1 interp2 : listO D -n> D) : listO D -n> D := λne Δ w,
-    (□ ∀ v, interp1 Δ v → WP App (of_val w) (of_val v) {{ interp2 Δ }})%I.
-  Solve Obligations with repeat intros ?; simpl; solve_proper.
-
-  Program Definition interp_forall
-      (interp_bound interp : listO D -n> D) : listO D -n> D := λne Δ w,
-    (□ ∀ τi : D,
-      ⌜∀ v, Persistent (τi v)⌝ → □ (∀ v, τi v -∗ interp_bound Δ v) → WP TApp (of_val w) {{ interp (τi :: Δ) }})%I.
-  Solve Obligations with repeat intros ?; simpl; solve_proper.
-
-  Program Definition interp_rec1
-      (interp : listO D -n> D) (Δ : listO D) (τi : D) : D := λne w,
-    (□ (∃ v, ⌜w = FoldV v⌝ ∧ ▷ interp (τi :: Δ) v))%I.
-
-  Global Instance interp_rec1_contractive
-    (interp : listO D -n> D) (Δ : listO D) : Contractive (interp_rec1 interp Δ).
-  Proof. by solve_contractive. Qed.
-
-  Lemma fixpoint_interp_rec1_eq (interp : listO D -n> D) Δ x :
-    fixpoint (interp_rec1 interp Δ) x ≡ interp_rec1 interp Δ (fixpoint (interp_rec1 interp Δ)) x.
-  Proof. exact: (fixpoint_unfold (interp_rec1 interp Δ) x). Qed.
-
-  Program Definition interp_rec (interp : listO D -n> D) : listO D -n> D := λne Δ,
-    fixpoint (interp_rec1 interp Δ).
+  Program Definition make_contractive (interp : listO D -df> D) : listO D -df> D :=
+    if domain_func_is_contractive interp then interp else
+      λdfco Δ, λdo w, (▷ interp Δ w)%I.
   Next Obligation.
-    intros interp n Δ1 Δ2 HΔ; apply fixpoint_ne => τi w. solve_proper.
+  Proof.
+    intros interp n ????; simpl.
+    apply later_contractive; destruct n; solve_proper.
   Qed.
 
-  Program Definition interp_ref_inv (l : loc) : D -n> iProp Σ := λne τi,
-    (∃ v, l ↦ᵢ v ∗ τi v)%I.
-  Solve Obligations with solve_proper.
+  Global Instance make_contractive_contractive interp :
+    Contractive (make_contractive interp).
+  Proof.
+    intros n ????.
+    rewrite /make_contractive.
+    destruct interp as [f [] Hf]; simpl in *.
+    - by apply Hf.
+    - apply later_contractive; destruct n; solve_proper.
+  Qed.
+
+  Program Definition env_lookup (x : var) : listO D -df> D :=
+    λdfne Δ, from_option id true_domain (Δ !! x).
+  Solve Obligations with simpl; solve_proper.
+
+  Program Definition interp_top : listO D -df> D := λdfco Δ, true_domain.
+  Next Obligation.
+  Proof. simpl; apply const_contractive. Qed.
+
+  Program Definition interp_unit : listO D -df> D := λdfco Δ, λdo w, (⌜w = UnitV⌝)%I.
+  Next Obligation.
+  Proof. done. Qed.
+
+  Program Definition interp_nat : listO D -df> D := λdfco Δ, λdo w, (⌜∃ n, w = #nv n⌝)%I.
+  Next Obligation.
+  Proof. done. Qed.
+
+  Program Definition interp_bool : listO D -df> D := λdfco Δ, λdo w, (⌜∃ n, w = #♭v n⌝)%I.
+  Next Obligation.
+  Proof. done. Qed.
+
+  Program Definition interp_prod
+      (interp1 interp2 : listO D -df> D) : listO D -df> D := λdfco Δ, λdo w,
+    (▷ ∃ w1 w2, ⌜w = PairV w1 w2⌝ ∧ interp1 Δ w1 ∧ interp2 Δ w2)%I.
+  Next Obligation.
+  Proof.
+    intros ???????; simpl.
+    apply later_contractive; destruct n; solve_proper.
+  Qed.
+
+  Program Definition interp_sum
+      (interp1 interp2 : listO D -df> D) : listO D -df> D := λdfco Δ, λdo w,
+    (▷ ((∃ w1, ⌜w = InjLV w1⌝ ∧ interp1 Δ w1) ∨
+        (∃ w2, ⌜w = InjRV w2⌝ ∧ interp2 Δ w2)))%I.
+  Next Obligation.
+  Proof.
+    intros ???????; simpl.
+    apply later_contractive; destruct n; try solve_proper.
+  Qed.
+
+  Program Definition interp_arrow
+      (interp1 interp2 : listO D -df> D) : listO D -df> D := λdfco Δ, λdo w,
+    (▷ (((∃ f, ⌜w = RecV f⌝) ∨ (∃ f, ⌜w = LamV f⌝)) ∧
+     □ ∀ v, interp1 Δ v → WP App (of_val w) (of_val v) {{ interp2 Δ }}))%I.
+  Next Obligation.
+  Proof.
+    intros ???????; simpl.
+    apply later_contractive; destruct n; try solve_proper.
+  Qed.
+
+  Program Definition interp_forall
+      (interp_bound interp : listO D -df> D) : listO D -df> D := λdfco Δ, λdo w,
+    (▷ ((∃ e, ⌜w = LamV e⌝) ∧
+        (□ ∀ τi : D,
+              ⌜∀ v, Persistent (τi v)⌝ → □ (∀ v, τi v -∗ interp_bound Δ v) →
+                    WP TApp (of_val w) {{ interp (τi :: Δ) }})))%I.
+  Next Obligation.
+  Proof.
+    intros ?????? Heq.
+    apply later_contractive; destruct n; solve_proper.
+  Qed.
+
+  Program Definition interp_rec1
+      (interp : listO D -df> D) (Δ : listO D) (τi : D) : D := λdo w,
+    (□ (∃ v, ⌜w = FoldV v⌝ ∧ make_contractive interp (τi :: Δ) v))%I.
+
+  Global Instance interp_rec1_contractive
+    (interp : listO D -df> D) (Δ : listO D) : Contractive (interp_rec1 interp Δ).
+  Proof.
+    intros ?????.
+    rewrite /interp_rec1; simpl.
+    apply intuitionistically_ne, exist_ne => ?.
+    apply and_ne; first done.
+    apply make_contractive_contractive.
+    destruct n; first done; simpl in *.
+    constructor; auto.
+    apply Reflexive_instance_0; auto.
+  Qed.
+
+  Program Definition interp_rec (interp : listO D -df> D) : listO D -df> D :=
+    λdfco Δ, λdo w, fixpoint (interp_rec1 interp Δ) w.
+  Next Obligation.
+    simpl.
+    intros interp n ? ? Heq ?; simpl.
+    rewrite fixpoint_unfold; simpl.
+    symmetry.
+    rewrite fixpoint_unfold; simpl.
+    symmetry.
+    apply intuitionistically_ne, exist_ne => ?.
+    apply and_ne; auto.
+    apply make_contractive_contractive.
+    destruct n; first done; simpl in *.
+    constructor; auto.
+    apply fixpoint_ne => z u.
+    rewrite /interp_rec1.
+    apply intuitionistically_ne, exist_ne => ?.
+    apply and_ne; auto.
+    f_equiv.
+    apply make_contractive_contractive.
+    apply dist_dist_later.
+    by constructor.
+  Qed.
 
   Program Definition interp_ref
-      (interp : listO D -n> D) : listO D -n> D := λne Δ w,
-    (∃ l, ⌜w = LocV l⌝ ∧ inv (logN .@ l) (interp_ref_inv l (interp Δ)))%I.
-  Solve Obligations with solve_proper.
+      (interp : listO D -df> D) : listO D -df> D := λdfco Δ, λdo w,
+    (∃ l, ⌜w = LocV l⌝ ∧ inv (logN .@ l) (∃ v, l ↦ᵢ v ∗ (interp Δ) v))%I.
+  Next Obligation.
+  Proof.
+    intros interp n ????; simpl.
+    apply exist_ne => ?.
+    apply and_ne; auto.
+    apply inv_contractive.
+    destruct n; solve_proper.
+  Qed.
 
-  Fixpoint interp (τ : type) : listO D -n> D :=
+  Fixpoint interp (τ : type) : listO D -df> D :=
     match τ return _ with
     | Top => interp_top
     | TUnit => interp_unit
@@ -97,78 +349,123 @@ Section logrel.
   Definition interp_expr (τ : type) (Δ : listO D) (e : expr) :
     iProp Σ := WP e {{ ⟦ τ ⟧ Δ }}%I.
 
-  Class env_Persistent Δ :=
-    env_persistent : Forall (λ τi, ∀ v, Persistent (τi v)) Δ.
-  Global Instance env_persistent_nil : env_Persistent [].
-  Proof. by constructor. Qed.
-  Global Instance env_persistent_cons τi Δ :
-    (∀ v, Persistent (τi v)) → env_Persistent Δ → env_Persistent (τi :: Δ).
-  Proof. by constructor. Qed.
-  Global Instance env_persistent_lookup Δ x v :
-    env_Persistent Δ → Persistent (env_lookup x Δ v).
-  Proof. intros HΔ; revert x; induction HΔ=>-[|?] /=; apply _. Qed.
-  Global Instance interp_persistent τ Δ v :
-    env_Persistent Δ → Persistent (interp τ Δ v).
-  Proof.
-    revert v Δ; induction τ=> v Δ HΔ; simpl; try apply _.
-    rewrite /Persistent fixpoint_interp_rec1_eq /interp_rec1 /= intuitionistically_into_persistently.
-    by apply persistently_intro'.
-  Qed.
   Global Instance interp_env_base_persistent Δ Γ vs :
-  env_Persistent Δ → TCForall Persistent (zip_with (λ τ, ⟦ τ ⟧ Δ) Γ vs).
+  TCForall Persistent (zip_with (λ τ, ⟦ τ ⟧ Δ) Γ vs).
   Proof.
-    intros HΔ. revert vs.
-    induction Γ => vs; simpl; destruct vs; constructor; apply _.
+    revert vs. induction Γ => vs; simpl; destruct vs; constructor; apply _.
   Qed.
-  Global Instance interp_env_persistent Γ Δ vs :
-    env_Persistent Δ → Persistent (⟦ Γ ⟧* Δ vs) := _.
+  Global Instance interp_env_persistent Γ Δ vs : Persistent (⟦ Γ ⟧* Δ vs) := _.
+
+  Lemma interp_weaken' Δ1 Π Δ2 τ :
+    ⟦ τ.[upn (length Δ1) (ren (+ length Π))] ⟧ (Δ1 ++ Π ++ Δ2)
+    ≡ ⟦ τ ⟧ (Δ1 ++ Δ2)
+    ∧ domain_func_is_contractive ⟦ τ.[upn (length Δ1) (ren (+ length Π))] ⟧ =
+      domain_func_is_contractive ⟦ τ ⟧.
+  Proof.
+    revert Δ1 Π Δ2. induction τ=> Δ1 Π Δ2; simpl; auto.
+    - split; last done.
+      intros w; simpl; properness; auto. by apply IHτ1. by apply IHτ2.
+    - split; last done.
+      intros w; simpl; properness; auto. by apply IHτ1. by apply IHτ2.
+    - split; last done.
+      intros w; simpl; properness; auto. by apply IHτ1. by apply IHτ2.
+    - split; last done.
+      intros ?; simpl; f_equiv.
+      apply fixpoint_proper=> τi w /=.
+      properness; auto.
+      rewrite /make_contractive.
+      destruct (IHτ (τi :: Δ1) Π Δ2) as [_ Hic].
+      rewrite /= -fold_up_upn in Hic.
+      rewrite Hic.
+      destruct domain_func_is_contractive.
+      + apply (IHτ (_ :: _)).
+      + simpl; apply later_proper.
+        apply (IHτ (_ :: _)).
+    - rewrite iter_up; destruct lt_dec as [Hl | Hl]; simpl.
+      { by rewrite !lookup_app_l. }
+      split; last done.
+      (* FIXME: Ideally we wouldn't have to do this kinf of surgery. *)
+      change (bi_ofeO (uPredI (iResUR Σ))) with (uPredO (iResUR Σ)).
+      rewrite !lookup_app_r; [|lia ..]. do 2 f_equiv. lia.
+    - split; last done.
+      intros w; simpl; properness; auto. by apply IHτ.
+      by apply (IHτ0 (_ :: _)).
+    - split; last done.
+      intros w; simpl; properness; auto. by apply IHτ.
+  Qed.
 
   Lemma interp_weaken Δ1 Π Δ2 τ :
     ⟦ τ.[upn (length Δ1) (ren (+ length Π))] ⟧ (Δ1 ++ Π ++ Δ2)
     ≡ ⟦ τ ⟧ (Δ1 ++ Δ2).
+  Proof. apply interp_weaken'. Qed.
+
+  Lemma trivial_subst n τ : upn n (τ .: ids) n = τ.[ren (+n)].
   Proof.
-    revert Δ1 Π Δ2. induction τ=> Δ1 Π Δ2; simpl; auto.
-    - intros w; simpl; properness; auto. by apply IHτ1. by apply IHτ2.
-    - intros w; simpl; properness; auto. by apply IHτ1. by apply IHτ2.
-    - intros w; simpl; properness; auto. by apply IHτ1. by apply IHτ2.
-    - apply fixpoint_proper=> τi w /=.
-      properness; auto. apply (IHτ (_ :: _)).
-    - rewrite iter_up; destruct lt_dec as [Hl | Hl]; simpl.
-      { by rewrite !lookup_app_l. }
-      (* FIXME: Ideally we wouldn't have to do this kinf of surgery. *)
-      change (bi_ofeO (uPredI (iResUR Σ))) with (uPredO (iResUR Σ)).
-      rewrite !lookup_app_r; [|lia ..]. do 2 f_equiv. lia.
-    - intros w; simpl; properness; auto. by apply IHτ.
-      by apply (IHτ0 (_ :: _)).
-    - intros w; simpl; properness; auto. by apply IHτ.
+    induction n; asimpl; first done.
+    by rewrite IHn; asimpl.
   Qed.
 
   Lemma interp_subst_up Δ1 Δ2 τ τ' :
+    valid_type τ →
     ⟦ τ ⟧ (Δ1 ++ interp τ' Δ2 :: Δ2)
-    ≡ ⟦ τ.[upn (length Δ1) (τ' .: ids)] ⟧ (Δ1 ++ Δ2).
+    ≡ ⟦ τ.[upn (length Δ1) (τ' .: ids)] ⟧ (Δ1 ++ Δ2)
+  ∧  (domain_func_is_contractive ⟦ τ.[upn (length Δ1) (τ' .: ids)] ⟧ ≠
+     domain_func_is_contractive ⟦ τ ⟧ →
+    τ = TVar (length Δ1)).
   Proof.
-    revert Δ1 Δ2; induction τ=> Δ1 Δ2; simpl; auto.
-    - intros w; simpl; properness; auto. by apply IHτ1. by apply IHτ2.
-    - intros w; simpl; properness; auto. by apply IHτ1. by apply IHτ2.
-    - intros w; simpl; properness; auto. by apply IHτ1. by apply IHτ2.
-    - apply fixpoint_proper=> τi w /=.
-      properness; auto. apply (IHτ (_ :: _)).
+    revert Δ1 Δ2; induction τ=> Δ1 Δ2 Hvl; simpl; try (split; (auto || done)).
+    - split; last done.
+      destruct Hvl as [Hvl1 Hvl2].
+      intros w; simpl; properness; auto. by apply IHτ1. by apply IHτ2.
+    - split; last done.
+      destruct Hvl as [Hvl1 Hvl2].
+      intros w; simpl; properness; auto. by apply IHτ1. by apply IHτ2.
+    - split; last done.
+      destruct Hvl as [Hvl1 Hvl2].
+      intros w; simpl; properness; auto. by apply IHτ1. by apply IHτ2.
+    - split; last done.
+      destruct Hvl as [Hvl1 Hvl2].
+      simpl in *.
+      intros ?; simpl; f_equiv.
+      apply fixpoint_proper=> τi w /=.
+      properness; auto.
+      rewrite /make_contractive.
+      destruct
+        (decide (domain_func_is_contractive
+                   ⟦ τ.[up (upn (length Δ1) (τ' .: ids))] ⟧
+                 = domain_func_is_contractive ⟦ τ ⟧)) as [->|Hneq].
+      + destruct (domain_func_is_contractive ⟦ τ ⟧).
+        * by apply (IHτ (_ :: _)).
+        * apply later_proper. by apply (IHτ (_ :: _)).
+      + by apply (IHτ (τi :: Δ1) Δ2) in Hneq; last done; subst.
     - rewrite iter_up; destruct lt_dec as [Hl | Hl]; simpl.
       { by rewrite !lookup_app_l. }
-      (* FIXME: Ideally we wouldn't have to do this kinf of surgery. *)
-      change (bi_ofeO (uPredI (iResUR Σ))) with (uPredO (iResUR Σ)).
-      rewrite !lookup_app_r; [|lia ..].
-      case EQ: (x - length Δ1) => [|n]; simpl.
-      { symmetry. asimpl. by rewrite (interp_weaken [] Δ1 Δ2 τ') . }
-      change (bi_ofeO (uPredI (iResUR Σ))) with (uPredO (iResUR Σ)).
-      rewrite !lookup_app_r; [|lia ..]. do 2 f_equiv. lia.
-    - intros w; simpl; properness; auto. by apply IHτ. apply (IHτ0 (_ :: _)).
-    - intros w; simpl; properness; auto. by apply IHτ.
+      split.
+      + (* FIXME: Ideally we wouldn't have to do this kinf of surgery. *)
+        change (bi_ofeO (uPredI (iResUR Σ))) with (uPredO (iResUR Σ)).
+        rewrite !lookup_app_r; [|lia ..].
+        case EQ: (x - length Δ1) => [|n]; simpl.
+        { symmetry. asimpl. by rewrite (interp_weaken [] Δ1 Δ2 τ'). }
+        change (bi_ofeO (uPredI (iResUR Σ))) with (uPredO (iResUR Σ)).
+        rewrite !lookup_app_r; [|lia ..]. do 2 f_equiv. lia.
+      + match goal with
+        | H : ¬ ?a < ?b |- _ => destruct (decide (a = b))
+        end; first by simplify_eq.
+        match goal with
+        | H : ¬ ?a < ?b |- _ => destruct (a - b) eqn:Heq
+        end; simpl; last done.
+        unfold var in *; lia.
+    - split; last done.
+      destruct Hvl as [Hvl1 Hvl2].
+      intros w; simpl; properness; auto. by apply IHτ. by apply (IHτ0 (_ :: _)).
+    - split; last done.
+      intros w; simpl; properness; auto. by apply IHτ.
   Qed.
 
   Lemma interp_subst Δ2 τ τ' v :
+    valid_type τ →
     ⟦ τ ⟧ (⟦ τ' ⟧ Δ2 :: Δ2) v ≡ ⟦ τ.[τ'/] ⟧ Δ2 v.
-  Proof. apply (interp_subst_up []). Qed.
+  Proof. by intros; apply (interp_subst_up []). Qed.
 
   Lemma interp_env_length Δ Γ vs : ⟦ Γ ⟧* Δ vs ⊢ ⌜length Γ = length vs⌝.
   Proof. by iIntros "[% ?]". Qed.
@@ -202,8 +499,8 @@ Section logrel.
   Qed.
 
   Definition interp_Tenv (Δ : listO D) (Ξ : list type) : iProp Σ:=
-    (⌜length Δ = length Ξ⌝ ∧ ∀ x τ, ⌜Ξ !! x = Some τ⌝ →
-                                    □ (∀ v, env_lookup x Δ v -∗ interp τ Δ v))%I.
+    (⌜length Δ = length Ξ⌝ ∧
+     ∀ x τ, ⌜Ξ !! x = Some τ⌝ → □ (∀ v, env_lookup x Δ v -∗ interp τ Δ v))%I.
 
   Lemma interp_Tenv_weaken Δ Ξ τ τi :
     □ (∀ v, τi v -∗ interp τ Δ v) ∧ interp_Tenv Δ Ξ
@@ -235,29 +532,53 @@ Section logrel.
       rewrite /= list_lookup_fmap Hσ //.
   Qed.
 
+  Lemma valid_rec_type τ :
+    valid_type (TRec τ) → domain_func_is_contractive ⟦ τ ⟧ = true.
+  Proof.
+    simpl; destruct τ; simpl; tauto.
+  Qed.
+
   Lemma logrel_subtyp Δ Ξ τ τ' v :
-    env_Persistent Δ →
     subtype Ξ τ τ' →
     interp_Tenv Δ Ξ ⊢ □ (interp τ Δ v -∗ interp τ' Δ v).
   Proof.
-    iIntros (HΔ Hsb) "#HΞ".
+    iIntros (Hsb) "#HΞ".
     iIntros "!# #Hτ".
-    iInduction Hsb as [] "IH" forall (Δ HΔ v) "HΞ Hτ"; simpl; auto.
+    iInduction Hsb as [] "IH" forall (Δ v) "HΞ Hτ"; simpl; auto.
     - iDestruct "HΞ" as "[% HΞ]".
       iApply ("HΞ" $! x); eauto.
     - iApply "IH1"; eauto.
       iAlways. iApply "IH"; eauto.
     - rewrite -/interp.
-      iAlways. iIntros (w) "#Hw".
+      iDestruct "Hτ" as "[? Hτ]".
+      iSplit; first done.
+      iNext.
+      iAlways.
+      iIntros (w) "#Hw".
       iApply wp_wand_r; iSplitL.
       + iApply "Hτ". iApply "IH"; eauto.
       + iIntros (?) "#?"; iApply "IH1"; eauto.
     - rewrite -/interp.
+      iNext.
+      iDestruct "Hτ" as "[? Hτ]".
+      iSplit; first done.
       iAlways. iIntros (τi Hτi) "#Hτi".
       iApply wp_wand_r; iSplitL; first by iApply "Hτ"; eauto.
       iIntros (?) "#?"; iApply "IH"; eauto.
-      + by iPureIntro; apply env_persistent_cons.
-      + iAlways. rewrite -interp_Tenv_weaken; auto.
+      iAlways. rewrite -interp_Tenv_weaken; auto.
+    - iLöb as "ILH" forall (v) "Hτ".
+      rewrite -> (fixpoint_unfold (interp_rec1 ⟦ τ ⟧ Δ)).
+      rewrite -> (fixpoint_unfold (interp_rec1 ⟦ σ ⟧ Δ)).
+      simpl.
+      iDestruct "Hτ" as (w Hw) "Hτ".
+      iAlways.
+      iExists _; iSplit; first done.
+      rewrite /make_contractive !valid_rec_type //.
+      iApply ("IH").
+      + iAlways.
+        rewrite -(interp_Tenv_weaken _ _ (TRec _)).
+        iSplit; last done.
+        iAlways. iIntros (?) "? /=".
   Qed.
 
 End logrel.
