typing.v
@@ -18,15 +18,84 @@ Instance Rename_type : Rename type. derive. Defined.
 Instance Subst_type : Subst type. derive. Defined.
 Instance SubstLemmas_typer : SubstLemmas type. derive. Qed.
 
+Fixpoint is_TVar τ :=
+  match τ with
+  | TVar _ => True
+  | _ => False
+  end.
+
+Lemma is_TVar_up_ren n m τ : is_TVar τ ↔ is_TVar τ.[upn n (ren (+m))].
+Proof.
+  revert n m; induction τ; intros n m; simpl; auto; [].
+  by rewrite iter_up; destruct lt_dec.
+Qed.
+
+Lemma valid_type_subst n σ τ : is_TVar τ.[upn n (σ .: ids)] → is_TVar τ.
+Proof. by destruct τ. Qed.
+
+Fixpoint valid_type (τ : type) :=
+  match τ with
+  | Top => True
+  | TUnit => True
+  | TNat => True
+  | TBool => True
+  | TProd τ1 τ2 => valid_type τ1 ∧ valid_type τ2
+  | TSum τ1 τ2 => valid_type τ1 ∧ valid_type τ2
+  | TArrow τ1 τ2 => valid_type τ1 ∧ valid_type τ2
+  | TRec τ => (¬ is_TVar τ) ∧ valid_type τ
+  | TVar x => True
+  | TForall σ τ => valid_type σ ∧ valid_type τ
+  | Tref τ => valid_type τ
+  end.
+
+Lemma valid_type_up_ren n m τ : valid_type τ → valid_type τ.[upn n (ren (+m))].
+Proof.
+  revert n m; induction τ; intros n m Hτ; simpl in *; try (by intuition auto).
+  - destruct Hτ as [Hτ1 Hτ2].
+    asimpl.
+    split; last by auto.
+    by rewrite -is_TVar_up_ren.
+  - by rewrite iter_up; destruct lt_dec.
+  - split; asimpl; intuition auto.
+Qed.
+
+Lemma valid_type_upn_subst n σ τ :
+  valid_type σ → valid_type τ → valid_type τ.[upn n (σ .: ids)].
+Proof.
+  revert n σ; induction τ; intros n σ Hσ Hτ; simpl in *;  asimpl;
+    try (by intuition auto).
+  - destruct Hτ as [Hτ1 Hτ2]; split; last by auto.
+    intros ?; apply Hτ1. eapply valid_type_subst; eauto.
+  - rewrite iter_up; destruct lt_dec; first done.
+    asimpl.
+    match goal with
+    | H : ¬ ?a < ?b |- _ => destruct (a - b)
+    end; last done.
+    asimpl.
+    by apply (valid_type_up_ren 0).
+Qed.
+
 Inductive subtype : list type → type → type → Prop :=
-| sbt_var Ξ x τ : Ξ !! x = Some τ → subtype Ξ (TVar x) τ
+| sbt_var Ξ x τ : valid_type τ → Ξ !! x = Some τ → subtype Ξ (TVar x) τ
 | sbt_refl Ξ τ : subtype Ξ τ τ
 | sbt_trans Ξ τ1 τ2 τ3 : subtype Ξ τ1 τ2 → subtype Ξ τ2 τ3 → subtype Ξ τ1 τ3
-| sbt_top Ξ τ : subtype Ξ τ Top
-| sbt_arrow Ξ σ σ' τ τ' : subtype Ξ σ' σ → subtype Ξ τ τ' →
-                        subtype Ξ (TArrow σ τ) (TArrow σ' τ')
-| sbt_forall Ξ σ τ1 τ2 : subtype (σ.[ren (+1)] :: (subst (ren (+1)) <$> Ξ)) τ1 τ2 →
-                         subtype Ξ (TForall σ τ1) (TForall σ τ2).
+| sbt_top Ξ τ : valid_type τ → subtype Ξ τ Top
+| sbt_arrow Ξ σ σ' τ τ' :
+    subtype Ξ σ' σ → subtype Ξ τ τ' →
+    subtype Ξ (TArrow σ τ) (TArrow σ' τ')
+| sbt_forall Ξ σ τ1 τ2 :
+    valid_type σ →
+    subtype (σ.[ren (+1)] :: (subst (ren (+1)) <$> Ξ)) τ1 τ2 →
+    subtype Ξ (TForall σ τ1) (TForall σ τ2)
+|sbt_rec Ξ σ τ :
+   valid_type (TRec σ) → valid_type (TRec τ) →
+   subtype ((TRec σ).[ren (+1)] :: (subst (ren (+1)) <$> Ξ)) σ τ →
+   subtype Ξ (TRec σ) (TRec τ).
+
+Lemma subtype_valid Ξ σ τ : subtype Ξ σ τ → valid_type σ ↔ valid_type τ.
+Proof.
+  induction 1; simpl in *; intuition auto.
+Qed.
 
 Fixpoint binop_res_type (op : binop) : type :=
   match op with
@@ -43,7 +112,7 @@ Inductive EqType : type → Prop :=
 Reserved Notation "Ξ |ₜ Γ ⊢ₜ e : τ" (at level 74, e, τ at next level).
 
 Inductive typed (Ξ Γ : list type) : expr → type → Prop :=
-  | Var_typed x τ : Γ !! x = Some τ → Ξ |ₜ Γ ⊢ₜ Var x : τ
+  | Var_typed x τ : valid_type τ → Γ !! x = Some τ → Ξ |ₜ Γ ⊢ₜ Var x : τ
   | Unit_typed : Ξ |ₜ Γ ⊢ₜ Unit : TUnit
   | Nat_typed n : Ξ |ₜ Γ ⊢ₜ #n n : TNat
   | Bool_typed b : Ξ |ₜ Γ ⊢ₜ #♭ b : TBool
@@ -55,8 +124,10 @@ Inductive typed (Ξ Γ : list type) : expr → type → Prop :=
   | Fst_typed e τ1 τ2 :
       Ξ |ₜ Γ ⊢ₜ e : TProd τ1 τ2 → Ξ |ₜ Γ ⊢ₜ Fst e : τ1
   | Snd_typed e τ1 τ2 : Ξ |ₜ Γ ⊢ₜ e : TProd τ1 τ2 → Ξ |ₜ Γ ⊢ₜ Snd e : τ2
-  | InjL_typed e τ1 τ2 : Ξ |ₜ Γ ⊢ₜ e : τ1 → Ξ |ₜ Γ ⊢ₜ InjL e : TSum τ1 τ2
-  | InjR_typed e τ1 τ2 : Ξ |ₜ Γ ⊢ₜ e : τ2 → Ξ |ₜ Γ ⊢ₜ InjR e : TSum τ1 τ2
+  | InjL_typed e τ1 τ2 :
+      valid_type τ2 → Ξ |ₜ Γ ⊢ₜ e : τ1 → Ξ |ₜ Γ ⊢ₜ InjL e : TSum τ1 τ2
+  | InjR_typed e τ1 τ2 :
+      valid_type τ1 → Ξ |ₜ Γ ⊢ₜ e : τ2 → Ξ |ₜ Γ ⊢ₜ InjR e : TSum τ1 τ2
   | Case_typed e0 e1 e2 τ1 τ2 τ3 :
      Ξ |ₜ Γ ⊢ₜ e0 : TSum τ1 τ2 → Ξ |ₜ τ1 :: Γ ⊢ₜ e1 : τ3 →
      Ξ |ₜ τ2 :: Γ ⊢ₜ e2 : τ3 → Ξ |ₜ Γ ⊢ₜ Case e0 e1 e2 : τ3
@@ -64,9 +135,10 @@ Inductive typed (Ξ Γ : list type) : expr → type → Prop :=
      Ξ |ₜ Γ ⊢ₜ e0 : TBool → Ξ |ₜ Γ ⊢ₜ e1 : τ → Ξ |ₜ Γ ⊢ₜ e2 : τ →
      Ξ |ₜ Γ ⊢ₜ If e0 e1 e2 : τ
   | Rec_typed e τ1 τ2 :
+      valid_type τ1 →
      Ξ |ₜ TArrow τ1 τ2 :: τ1 :: Γ ⊢ₜ e : τ2 → Ξ |ₜ Γ ⊢ₜ Rec e : TArrow τ1 τ2
   | Lam_typed e τ1 τ2 :
-      Ξ |ₜ τ1 :: Γ ⊢ₜ e : τ2 → Ξ |ₜ Γ ⊢ₜ Lam e : TArrow τ1 τ2
+      valid_type τ1 → Ξ |ₜ τ1 :: Γ ⊢ₜ e : τ2 → Ξ |ₜ Γ ⊢ₜ Lam e : TArrow τ1 τ2
   | LetIn_typed e1 e2 τ1 τ2 :
       Ξ |ₜ Γ ⊢ₜ e1 : τ1 → Ξ |ₜ τ1 :: Γ ⊢ₜ e2 : τ2 → Ξ |ₜ Γ ⊢ₜ LetIn e1 e2 : τ2
   | Seq_typed e1 e2 τ1 τ2 :
@@ -74,11 +146,15 @@ Inductive typed (Ξ Γ : list type) : expr → type → Prop :=
   | App_typed e1 e2 τ1 τ2 :
      Ξ |ₜ Γ ⊢ₜ e1 : TArrow τ1 τ2 → Ξ |ₜ Γ ⊢ₜ e2 : τ1 → Ξ |ₜ Γ ⊢ₜ App e1 e2 : τ2
   | TLam_typed e σ τ :
+      valid_type σ →
      σ.[ren (+1)] :: (subst (ren (+1)) <$> Ξ) |ₜ subst (ren (+1)) <$> Γ ⊢ₜ e : τ →
      Ξ |ₜ Γ ⊢ₜ TLam e : TForall σ τ
-  | TApp_typed e σ τ τ' : Ξ |ₜ Γ ⊢ₜ e : TForall σ τ → subtype Ξ τ' σ →
+  | TApp_typed e σ τ τ' :
+      valid_type σ →
+      Ξ |ₜ Γ ⊢ₜ e : TForall σ τ → subtype Ξ τ' σ →
       Ξ |ₜ Γ ⊢ₜ TApp e : τ.[τ'/]
-  | TFold e τ : Ξ |ₜ Γ ⊢ₜ e : τ.[TRec τ/] → Ξ |ₜ Γ ⊢ₜ Fold e : TRec τ
+  | TFold e τ :
+      valid_type (TRec τ) → Ξ |ₜ Γ ⊢ₜ e : τ.[TRec τ/] → Ξ |ₜ Γ ⊢ₜ Fold e : TRec τ
   | TUnfold e τ : Ξ |ₜ Γ ⊢ₜ e : TRec τ → Ξ |ₜ Γ ⊢ₜ Unfold e : τ.[TRec τ/]
   | TFork e : Ξ |ₜ Γ ⊢ₜ e : TUnit → Ξ |ₜ Γ ⊢ₜ Fork e : TUnit
   | TAlloc e τ : Ξ |ₜ Γ ⊢ₜ e : τ → Ξ |ₜ Γ ⊢ₜ Alloc e : Tref τ
@@ -91,113 +167,12 @@ Inductive typed (Ξ Γ : list type) : expr → type → Prop :=
   | TSub e τ τ' : Ξ |ₜ Γ ⊢ₜ e : τ → subtype Ξ τ τ' → Ξ |ₜ Γ ⊢ₜ e : τ'
 where "Ξ |ₜ Γ ⊢ₜ e : τ" := (typed Ξ Γ e τ).
 
-(* Lemma typed_subst_invariant Ξ Γ e τ s1 s2 : *)
-(*   Ξ |ₜ Γ ⊢ₜ e : τ → (∀ x, x < length Γ → s1 x = s2 x) → e.[s1] = e.[s2]. *)
-(* Proof. *)
-(*   intros Htyped; revert s1 s2. *)
-(*   assert (∀ x Γ, x < length (subst (ren (+1)) <$> Γ) → x < length Γ). *)
-(*   { intros ??. by rewrite fmap_length. } *)
-(*   assert (∀ {A} `{Ids A} `{Rename A} (s1 s2 : nat → A) x, *)
-(*     (x ≠ 0 → s1 (pred x) = s2 (pred x)) → up s1 x = up s2 x). *)
-(*   { intros A H1 H2. rewrite /up=> s1 s2 [|x] //=; auto with f_equal lia. } *)
-(*   induction Htyped => s1 s2 Hs; f_equal/=; eauto using lookup_lt_Some with lia. *)
-(* Qed. *)
-(* Lemma n_closed_invariant n (e : expr) s1 s2 : *)
-(*   (∀ f, e.[upn n f] = e) → (∀ x, x < n → s1 x = s2 x) → e.[s1] = e.[s2]. *)
-(* Proof. *)
-(*   intros Hnc. specialize (Hnc (ren (+1))). *)
-(*   revert n Hnc s1 s2. *)
-(*   induction e => m Hmc s1 s2 H1; asimpl in *; try f_equal; *)
-(*     try (match goal with H : _ |- _ => eapply H end; eauto; *)
-(*          try inversion Hmc; try match goal with H : _ |- _ => by rewrite H end; *)
-(*          fail). *)
-(*   - apply H1. rewrite iter_up in Hmc. destruct lt_dec; try lia. *)
-(*     asimpl in *. injection Hmc as Hmc. unfold var in *. omega. *)
-(*   - unfold upn in *. *)
-(*     change (e.[up (up (upn m (ren (+1))))]) with *)
-(*     (e.[iter (S (S m)) up (ren (+1))]) in *. *)
-(*     apply (IHe (S (S m))). *)
-(*     + inversion Hmc; match goal with H : _ |- _ => (by rewrite H) end. *)
-(*     + intros [|[|x]] H2; [by cbv|by cbv |]. *)
-(*       asimpl; rewrite H1; auto with lia. *)
-(*   - apply (IHe (S m)). *)
-(*     + inversion Hmc; match goal with H : _ |- _ => (by rewrite H) end. *)
-(*     + intros [|x] H2; [by cbv |]. *)
-(*       asimpl; rewrite H1; auto with lia. *)
-(*   - apply (IHe0 (S m)). *)
-(*     + inversion Hmc; match goal with H : _ |- _ => (by rewrite H) end. *)
-(*     + intros [|x] H2; [by cbv |]. *)
-(*       asimpl; rewrite H1; auto with lia. *)
-(*   - change (e1.[up (upn m (ren (+1)))]) with *)
-(*     (e1.[iter (S m) up (ren (+1))]) in *. *)
-(*     apply (IHe0 (S m)). *)
-(*     + inversion Hmc; match goal with H : _ |- _ => (by rewrite H) end. *)
-(*     + intros [|x] H2; [by cbv |]. *)
-(*       asimpl; rewrite H1; auto with lia. *)
-(*   - change (e2.[up (upn m (ren (+1)))]) with *)
-(*     (e2.[upn (S m) (ren (+1))]) in *. *)
-(*     apply (IHe1 (S m)). *)
-(*     + inversion Hmc; match goal with H : _ |- _ => (by rewrite H) end. *)
-(*     + intros [|x] H2; [by cbv |]. *)
-(*       asimpl; rewrite H1; auto with lia. *)
-(* Qed. *)
-
-Fixpoint env_subst (vs : list val) : var → expr :=
-  match vs with
-  | [] => ids
-  | v :: vs' => (of_val v) .: env_subst vs'
-  end.
-
-Lemma env_subst_lookup vs x v :
-  vs !! x = Some v → env_subst vs x = of_val v.
+Lemma typed_valid Ξ Γ e τ : Ξ |ₜ Γ ⊢ₜ e : τ → valid_type τ.
 Proof.
-  revert vs; induction x => vs.
-  - by destruct vs; inversion 1.
-  - destruct vs as [|w vs]; first by inversion 1.
-    rewrite -lookup_tail /=.
-    apply IHx.
+  induction 1; simpl in *; intuition auto.
+  - match goal with op : binop |- _ => by destruct op end.
+  - apply (valid_type_upn_subst 0); auto.
+    by rewrite subtype_valid; last by eauto.
+  - by apply (valid_type_upn_subst 0).
+  - rewrite -subtype_valid; eauto.
 Qed.
-
-(* Lemma typed_n_closed Γ τ e : Γ ⊢ₜ e : τ → (∀ f, e.[upn (length Γ) f] = e). *)
-(* Proof. *)
-(*   intros H. induction H => f; asimpl; simpl in *; auto with f_equal. *)
-(*   - apply lookup_lt_Some in H. rewrite iter_up. destruct lt_dec; auto with lia. *)
-(*   - f_equal. apply IHtyped. *)
-(*   - by f_equal; rewrite map_length in IHtyped. *)
-(* Qed. *)
-
-(** Weakening *)
-(* Lemma context_gen_weakening ξ Γ' Γ e τ : *)
-(*   Γ' ++ Γ ⊢ₜ e : τ → *)
-(*   Γ' ++ ξ ++ Γ ⊢ₜ e.[upn (length Γ') (ren (+ (length ξ)))] : τ. *)
-(* Proof. *)
-(*   intros H1. *)
-(*   remember (Γ' ++ Γ) as Ξ. revert Γ' Γ ξ HeqΞ. *)
-(*   induction H1 => Γ1 Γ2 ξ HeqΞ; subst; asimpl in *; eauto using typed. *)
-(*   - rewrite iter_up; destruct lt_dec as [Hl | Hl]. *)
-(*     + constructor. rewrite lookup_app_l; trivial. by rewrite lookup_app_l in H. *)
-(*     + asimpl. constructor. rewrite lookup_app_r; auto with lia. *)
-(*       rewrite lookup_app_r; auto with lia. *)
-(*       rewrite lookup_app_r in H; auto with lia. *)
-(*       match goal with *)
-(*         |- _ !! ?A = _ => by replace A with (x - length Γ1) by lia *)
-(*       end. *)
-(*   - econstructor; eauto. by apply (IHtyped2 (_::_)). by apply (IHtyped3 (_::_)). *)
-(*   - constructor. by apply (IHtyped (_ :: _ :: _)). *)
-(*   - constructor. by apply (IHtyped (_ :: _)). *)
-(*   - econstructor; eauto. by apply (IHtyped2 (_::_)). *)
-(*   - constructor. *)
-(*     specialize (IHtyped *)
-(*       (subst (ren (+1)) <$> Γ1) (subst (ren (+1)) <$> Γ2) (subst (ren (+1)) <$> ξ)). *)
-(*     asimpl in *. rewrite ?map_length in IHtyped. *)
-(*     repeat rewrite fmap_app. apply IHtyped. *)
-(*     by repeat rewrite fmap_app. *)
-(* Qed. *)
-
-(* Lemma context_weakening ξ Γ e τ : *)
-(*   Γ ⊢ₜ e : τ → ξ ++ Γ ⊢ₜ e.[(ren (+ (length ξ)))] : τ. *)
-(* Proof. eapply (context_gen_weakening _ []). Qed. *)
-
-(* Lemma closed_context_weakening ξ Γ e τ : *)
-(*   (∀ f, e.[f] = e) → Γ ⊢ₜ e : τ → ξ ++ Γ ⊢ₜ e : τ. *)
-(* Proof. intros H1 H2. erewrite <- H1. by eapply context_weakening. Qed. *)
